Add lemmas about state; start fixing memory invariant

coq/LLVMGen/Init.v
@@ -290,6 +290,20 @@ Proof.
     now rewrite app_nil_r.
 Qed.
 
+Ltac fold_initIRGlobals_rev :=
+  repeat match goal with
+         | [H : context[init_with_data initOneIRGlobal global_uniq_chk ?l ?globals ?s] |- _ ] =>
+           replace (init_with_data initOneIRGlobal global_uniq_chk l globals s)
+             with (initIRGlobals_rev l globals s)
+             in *
+             by reflexivity
+         | [|- context[init_with_data initOneIRGlobal global_uniq_chk ?l ?globals ?s]] =>
+           replace (init_with_data initOneIRGlobal global_uniq_chk l globals s)
+             with (initIRGlobals_rev l globals s)
+             in *
+             by reflexivity
+         end.
+
 Lemma initIRGlobals_inl
       (data : list binary64)
       (globals : list (string * DSHType))
@@ -689,20 +703,27 @@ Proof.
   reflexivity.
 Qed.
 
+Definition addVar (a : string * DSHType) (s : IRState) : IRState :=
+  let '(nm, t) := a in
+  {| block_count := block_count s;
+     local_count := local_count s;
+     void_count := void_count s;
+     Γ := (ID_Global (Name nm), TYPE_Pointer (getIRType t)) :: Γ s |}.
 
-Fact initOneIRGlobal_state_change:
-  forall data nm t g' i0 i1 r,
-    initOneIRGlobal data (nm,t) i0 ≡ inr (i1, (g', r))
-    -> inr (i1,()) ≡ (addVars [(ID_Global (Name nm), TYPE_Pointer (getIRType t))]) i0.
+Lemma initOneIRGlobal_state_change
+      (data0 data1 : list binary64)
+      (a : string * DSHType)
+      (s0 s1 : IRState)
+      r
+  :
+    initOneIRGlobal data0 a s0 ≡ inr (s1, (data1, r))
+    -> s1 ≡ addVar a s0.
 Proof.
-  intros data nm t g' i0 i1 r H.
-  unfold initOneIRGlobal in H.
-  destruct t.
-  - break_let.
-    inv H.
-    reflexivity.
-  - break_let; cbn in H; inl_inr_inv; reflexivity.
-  - break_let; cbn in H; inl_inr_inv; reflexivity.
+  intros.
+  destruct a.
+  cbn in *.
+  repeat break_match.
+  all: now invc H.
 Qed.
 
 Lemma getStateVar_preserves_st
@@ -1194,19 +1215,19 @@ Proof.
   - cbn. rewrite IHg1. now subst.
 Qed.
 
-Lemma init_with_data_app_global_uniq_chk
+Lemma initIRGlobals_rev_app_inv
       (pre post : list (string * DSHType))
       (s0 s1 : IRState)
       (l0 l1 : list binary64)
       (g : list (toplevel_entity typ (LLVMAst.block typ * list (LLVMAst.block typ)))) 
   :
-    init_with_data initOneIRGlobal
-                   global_uniq_chk l0 (pre ++ post) s0 ≡ inr (s1, (l1, g)) →
+    initIRGlobals_rev l0 (pre ++ post) s0 ≡ inr (s1, (l1, g)) →
     ∃ l' s' g1 g2,
-      init_with_data initOneIRGlobal global_uniq_chk l0 pre s0 ≡ inr (s', (l', g1)) ∧
-      init_with_data initOneIRGlobal global_uniq_chk l' post s' ≡ inr (s1, (l1, g2)) ∧
+      initIRGlobals_rev l0 pre s0 ≡ inr (s', (l', g1)) ∧
+      initIRGlobals_rev l' post s' ≡ inr (s1, (l1, g2)) ∧
       g ≡ g1 ++ g2.
 Proof.
+  unfold initIRGlobals_rev.
   dependent induction pre; intros A.
   -
     intros.
@@ -1320,18 +1341,19 @@ Proof.
   lia.
 Qed.
 
-Lemma init_with_data_app_global_uniq_chk_inv
+Lemma initIRGlobals_rev_app
       (pre post : list (string * DSHType))
       (s0 s' s1 : IRState)
       (l0 l' l1 : list binary64)
       (g1 g2 : list (toplevel_entity typ (LLVMAst.block typ * list (LLVMAst.block typ))))
   :
     list_uniq fst (pre ++ post) ->
-    init_with_data initOneIRGlobal global_uniq_chk l0 pre s0 ≡ inr (s', (l', g1)) ->
-    init_with_data initOneIRGlobal global_uniq_chk l' post s' ≡ inr (s1, (l1, g2)) ->
-    init_with_data initOneIRGlobal global_uniq_chk l0 (pre ++ post) s0
+    initIRGlobals_rev l0 pre s0 ≡ inr (s', (l', g1)) ->
+    initIRGlobals_rev l' post s' ≡ inr (s1, (l1, g2)) ->
+    initIRGlobals_rev l0 (pre ++ post) s0
     ≡ inr (s1, (l1, g1 ++ g2)).
 Proof.
+  unfold initIRGlobals_rev.
   intros.
   dependent induction pre.
   -
@@ -1470,11 +1492,6 @@ Proof.
   reflexivity.
 Qed.
 
-Ltac destruct_unit :=
-  repeat match goal with
-         | [x : unit |- _] => destruct x
-         end.
-
 Lemma initOneIRGlobal_some_g_exp
       (data data' : list binary64)
       (nmt : string * DSHType)
@@ -1595,7 +1612,7 @@ Proof.
     reflexivity.
   -
     rewrite list_cons_app in I.
-    apply init_with_data_app_global_uniq_chk in I.
+    apply initIRGlobals_rev_app_inv in I.
     destruct I as (data' & s' & g1 & g2 & I1 & I2 & G).
     copy_apply initIRGlobals_rev_Γ_len I1; rename H into L1.
     copy_apply initIRGlobals_rev_Γ_len I2; rename H into L2.
@@ -1688,6 +1705,145 @@ Proof.
   erewrite initIRGlobals_Γ_preserved by eassumption.
   reflexivity.
 Qed.
+
+Definition append_globals_rev
+           (globals : list (string * DSHType))
+           (s : IRState)
+  : IRState :=
+  {| block_count := block_count s;
+     local_count := local_count s;
+     void_count := void_count s;
+     Γ := map IR_of_global (rev globals) ++ (Γ s) |}.
+
+Lemma initIRGlobals_rev_state_change
+      (globals : list (string * DSHType))
+      (data0 data1 : list binary64)
+      (s0 s1 : IRState)
+      ginit
+  :
+    initIRGlobals_rev data0 globals s0 ≡ inr (s1, (data1, ginit)) ->
+    s1 ≡ append_globals_rev globals s0.
+Proof.
+  intros.
+  destruct s1.
+  unfold append_globals_rev.
+  f_equal.
+  4: apply initIRGlobals_rev_Γ in H; assumption.
+  all: dependent induction globals; [now invc H |].
+  all: cbn in *.
+  all: repeat break_match; invc H.
+  all: copy_apply global_uniq_chk_preserves_st Heqs; subst i.
+  all: copy_apply initOneIRGlobal_state_change Heqs0; subst i0.
+  all: apply IHglobals in Heqs1.
+  all: subst.
+  all: unfold addVar; break_let; reflexivity.
+Qed.
+
+Lemma initOneIRglobal_state_writer
+      (data0 data1 : list binary64)
+      (s0 s1 : IRState)
+      (a : string * DSHType)
+      (r : toplevel_entity typ (LLVMAst.block typ * list (LLVMAst.block typ)))
+  :
+    initOneIRGlobal data0 a s0 ≡ inr (s1, (data1, r)) →
+    forall s',
+      initOneIRGlobal data0 a s' ≡ inr (addVar a s', (data1, r)).
+Proof.
+  intros.
+  destruct a.
+  cbn in *.
+  repeat break_match.
+  all: now invc H.
+Qed.
+
+Lemma initIRGlobals_state_writer
+      (globals : list (string * DSHType))
+      (s0 s1 : IRState)
+      (data0 data1 : list binary64)
+      (g : list (toplevel_entity typ (LLVMAst.block typ * list (LLVMAst.block typ)))) 
+  :
+    initIRGlobals_rev data0 globals s0 ≡ inr (s1, (data1, g)) →
+    forall s',
+      initIRGlobals_rev data0 globals s' ≡ inr (append_globals_rev globals s', (data1, g)).
+Proof.
+  unfold append_globals_rev.
+  dependent induction globals; intros I s'; cbn in *.
+  -
+    invc I.
+    now destruct s'.
+  -
+    break_match_goal; break_match_hyp; try congruence.
+    { (* [global_uniq_chk] inconsistent *)
+      exfalso; clear - Heqs Heqs2.
+      unfold global_uniq_chk in *.
+      destruct (assert_false_to_err ("duplicate global name: " @@ fst a)
+                                    (globals_name_present (fst a) globals) ()).
+      all: cbn in *; congruence.
+    }
+    repeat break_let; subst.
+
+    break_match_goal; break_match_hyp; try congruence.
+    { (* [initOnrIRGlobal] inconsistent *)
+      exfalso; clear - Heqs1 Heqs2.
+      destruct a.
+      cbn in *.
+      repeat break_match; congruence.
+    }
+    repeat break_let; subst.
+
+    copy_apply global_uniq_chk_preserves_st Heqs0; subst i.
+    copy_apply global_uniq_chk_preserves_st Heqs; subst i0.
+    repeat destruct_unit.
+    copy_apply initOneIRGlobal_state_change Heqs1; subst i2.
+    copy_apply initOneIRGlobal_state_change Heqs2; subst i1.
+
+    apply initOneIRglobal_state_writer with (s':=s') in Heqs2.
+    rewrite Heqs1 in Heqs2.
+    inversion Heqs2; clear Heqs2; subst l0 t0.
+    break_match_goal; break_match_hyp; try congruence.
+    { (* [init_with_data] inconsistent *)
+      exfalso.
+      repeat break_let; subst.
+      inversion I; clear I; subst i l0.
+      fold_initIRGlobals_rev.
+      apply IHglobals with (s':=addVar a s') in Heqs3.
+      congruence.
+    }
+    repeat break_let; subst.
+    invc I.
+    apply IHglobals with (s':=addVar a s') in Heqs3.
+    fold_initIRGlobals_rev.
+    rewrite Heqs2 in Heqs3.
+    invc Heqs3.
+    unfold addVar.
+    destruct a.
+    cbn.
+    f_equal.
+    rewrite map_app; rewrite <-app_assoc; reflexivity.
+Qed.
+
+Ltac dedup_states :=
+  repeat match goal with
+         | [ H : global_uniq_chk _ _ _ ≡ inr (?s, _) |- _] =>
+           copy_apply global_uniq_chk_preserves_st H; subst s
+         | [ H : initOneIRGlobal _ _ _ ≡ inr (?s, _) |- _] =>
+           copy_apply initOneIRGlobal_state_change H; subst s
+         | [ H : initIRGlobals_rev _ _ _ ≡ inr (?s, _) |- _] =>
+           copy_apply initIRGlobals_rev_state_change H; subst s
+         end.
+
+Lemma initIRGlobals_app_inv
+      (pre post : list (string * DSHType))
+      (s0 s1 : IRState)
+      (l0 l1 : list binary64)
+      (g : list (toplevel_entity typ (LLVMAst.block typ * list (LLVMAst.block typ)))) 
+  :
+    initIRGlobals l0 (pre ++ post) s0 ≡ inr (s1, (l1, g)) →
+    ∃ l' s' g1 g2,
+      initIRGlobals l0 pre s0 ≡ inr (s', (l', g1)) ∧
+      initIRGlobals l' post s' ≡ inr (s1, (l1, g2)) ∧
+      g ≡ g1 ++ g2.
+Abort.
 
 (** [memory_invariant] relation must holds after initialization of global variables *)
 Lemma memory_invariant_after_init
@@ -1837,7 +1993,8 @@ Proof.
                  TYPE_Pointer (TYPE_Array (Z.to_N (Int64.intval i)) TYPE_Double));
                 (ID_Global (Anon 1%Z), TYPE_Array (Z.to_N (Int64.intval o)) TYPE_Double);
                 (ID_Global (Anon 0%Z), TYPE_Array (Z.to_N (Int64.intval i)) TYPE_Double)] as v.
-    induction globals; intros v gdecls data data' H.
+    generalize dependent s1.
+    induction globals; intros s v gdecls data data' H.
     -
       cbn in *.
       inl_inr_inv.
@@ -1845,14 +2002,14 @@ Proof.
     -
       cbn in H.
       repeat break_match_hyp; try inl_inr.
-      (*
-      apply global_uniq_chk_preserves_st in Heqs; subst i0.
-      inl_inr_inv; subst.
+      apply global_uniq_chk_preserves_st in Heqs1; subst i1.
+      repeat inl_inr_inv; subst.
+      invc H3.
       cbn.
       apply ListUtil.app_nil.
       +
-        clear - Heqs0.
-        rename Heqs0 into H.
+        clear - Heqs2.
+        rename Heqs2 into H.
         unfold initOneIRGlobal in H.
         cbn in *.
         repeat break_match.
@@ -1860,17 +2017,17 @@ Proof.
         all: reflexivity.
       +
         destruct a.
-        apply initOneIRGlobal_state_change in Heqs0; cbn in Heqs0; inl_inr_inv.
-        destruct i1.
-        inversion H0.
+        copy_apply initOneIRGlobal_state_change Heqs2; subst i2.
         erewrite IHglobals with
             (data:=l)
             (data':=data')
             (v:=(ID_Global (Name s), TYPE_Pointer (getIRType d)) :: v)
         ; clear IHglobals; try reflexivity.
 
-        subst Γ. subst.
-        apply Heqs1.
+        fold_initIRGlobals_rev.
+        unfold addVar in *; cbn in *.
+        rewrite Heqs3.
+        reflexivity.
   }
   replace (flat_map (declarations_of typ) gdecls) with (@nil (declaration typ)) in *.
   2:{
@@ -1895,8 +2052,8 @@ Proof.
                  TYPE_Pointer (TYPE_Array (Z.to_N (Int64.intval i)) TYPE_Double));
                 (ID_Global (Anon 1%Z), TYPE_Array (Z.to_N (Int64.intval o)) TYPE_Double);
                 (ID_Global (Anon 0%Z), TYPE_Array (Z.to_N (Int64.intval i)) TYPE_Double)] as v.
-
-    induction globals; intros v gdecls data data' H.
+    generalize dependent s1.
+    induction globals; intros s v gdecls data data' H.
     -
       cbn in *.
       inl_inr_inv.
@@ -1904,13 +2061,14 @@ Proof.
     -
       cbn in H.
       repeat break_match_hyp; try inl_inr.
-      apply global_uniq_chk_preserves_st in Heqs; subst i0.
-      inl_inr_inv; subst.
+      apply global_uniq_chk_preserves_st in Heqs1; subst i1.
+      repeat inl_inr_inv; subst.
+      invc H3.
       cbn.
       apply ListUtil.app_nil.
       +
-        clear - Heqs0.
-        rename Heqs0 into H.
+        clear - Heqs2.
+        rename Heqs2 into H.
         unfold initOneIRGlobal in H.
         cbn in *.
         repeat break_match.
@@ -1918,17 +2076,17 @@ Proof.
         all: reflexivity.
       +
         destruct a.
-        apply initOneIRGlobal_state_change in Heqs0; cbn in Heqs0; inl_inr_inv.
-        destruct i1.
-        inversion H0.
+        copy_apply initOneIRGlobal_state_change Heqs2; subst i2.
         erewrite IHglobals with
             (data:=l)
             (data':=data')
             (v:=(ID_Global (Name s), TYPE_Pointer (getIRType d)) :: v)
         ; clear IHglobals; try reflexivity.
 
-        subst Γ. subst.
-        apply Heqs1.
+        fold_initIRGlobals_rev.
+        unfold addVar in *; cbn in *.
+        rewrite Heqs3.
+        reflexivity.
   }
   replace (flat_map (definitions_of typ) gdecls)
     with (@nil (definition typ (LLVMAst.block typ * list (LLVMAst.block typ))))
@@ -1955,8 +2113,8 @@ Proof.
                  TYPE_Pointer (TYPE_Array (Z.to_N (Int64.intval i)) TYPE_Double));
                 (ID_Global (Anon 1%Z), TYPE_Array (Z.to_N (Int64.intval o)) TYPE_Double);
                 (ID_Global (Anon 0%Z), TYPE_Array (Z.to_N (Int64.intval i)) TYPE_Double)] as v.
-
-    induction globals; intros v gdecls data data' H.
+    generalize dependent s1.
+    induction globals; intros s v gdecls data data' H.
     -
       cbn in *.
       inl_inr_inv.
@@ -1964,13 +2122,14 @@ Proof.
     -
       cbn in H.
       repeat break_match_hyp; try inl_inr.
-      apply global_uniq_chk_preserves_st in Heqs; subst i0.
-      inl_inr_inv; subst.
+      apply global_uniq_chk_preserves_st in Heqs1; subst i1.
+      repeat inl_inr_inv; subst.
+      invc H3.
       cbn.
       apply ListUtil.app_nil.
       +
-        clear - Heqs0.
-        rename Heqs0 into H.
+        clear - Heqs2.
+        rename Heqs2 into H.
         unfold initOneIRGlobal in H.
         cbn in *.
         repeat break_match.
@@ -1978,17 +2137,17 @@ Proof.
         all: reflexivity.
       +
         destruct a.
-        apply initOneIRGlobal_state_change in Heqs0; cbn in Heqs0; inl_inr_inv.
-        destruct i1.
-        inversion H0.
+        copy_apply initOneIRGlobal_state_change Heqs2; subst i2.
         erewrite IHglobals with
             (data:=l)
             (data':=data')
             (v:=(ID_Global (Name s), TYPE_Pointer (getIRType d)) :: v)
         ; clear IHglobals; try reflexivity.
 
-        subst Γ. subst.
-        apply Heqs1.
+        fold_initIRGlobals_rev.
+        unfold addVar in *; cbn in *.
+        rewrite Heqs3.
+        reflexivity.
   }
 
   repeat rewrite app_nil_r.
@@ -2221,18 +2380,11 @@ Proof.
       enough (
           forall pre post gdecls1 gdecls2 s' l',
             globals ≡ pre ++ post -> 
-
             gdecls ≡ gdecls1 ++ gdecls2 ->
-
-            init_with_data initOneIRGlobal
-                           global_uniq_chk l1 pre s_yx ≡ inr (s', (l', gdecls1)) ->
-
-            init_with_data initOneIRGlobal
-                           global_uniq_chk l' post s' ≡ inr (s1, (l2, gdecls2)) ->
-
+            initIRGlobals_rev l1 pre s_yx ≡ inr (s', (l', gdecls1)) ->
+            initIRGlobals_rev l' post s' ≡ inr (s1, (l2, gdecls2)) ->
             allocated_globals_mcfg pre (mg, ())
                                       (m, (le0, stack0, (g, ()))) ->
-
             eutt (allocated_globals_mcfg (pre ++ post))
                  (Ret (mg, ()))
                     (interp_mcfg
@@ -2240,9 +2392,11 @@ Proof.
                                    (map (Fmap_global typ dtyp (typ_to_dtyp []))
                                         (flat_map (globals_of typ) gdecls2)))
                        g (le0, stack0) m)).
+      (*
       {
         replace (globals) with ([] ++ globals) in * by reflexivity.
-        apply init_with_data_app_global_uniq_chk in LG.
+        apply initIRGlobals_inr in LG.
+        apply initIRGlobals_rev_app_inv in LG.
         destruct LG as (l' & s' & gdecls1 & gdecls2 & PRE & POST & GDECLS).
         specialize (H0 [] globals gdecls1 gdecls2 s' l').
         full_autospecialize H0; try congruence.
@@ -2937,6 +3091,7 @@ Proof.
       rewrite Eq.bind_ret_l.
        *)
       admit.
+*)
 Abort.
 
 (* with init step  *)
@@ -3282,5 +3437,4 @@ Hint Rewrite interp_to_L3_ret : local.
 
 
     (*         unfold global_YX,constArray in EQ1. *)
-*)
 Abort.
